WIP

cfrontend/CtypesC.v
@@ -2,15 +2,85 @@ Require Import Axioms CoqlibC Maps Errors.
 Require Import AST Linking.
 Require Archi.
 
-Require Export Ctypes.
+Require Export Ctypes Csem Csyntax ASTC.
+Require Import Errors.
+Require Import sflib.
+Require Import Skeleton ASTC.
 
 Set Implicit Arguments.
 
-Definition fundef_of_fundef F (f: fundef F): AST.fundef F :=
+Definition fundef_of_fundef F (f: Ctypes.fundef F): AST.fundef F :=
   match f with
   | Internal f => AST.Internal f
   | External ef _ _ _ => AST.External ef
   end
 .
 
-Coercion fundef_of_fundef: fundef >-> AST.fundef.
+Coercion fundef_of_fundef: Ctypes.fundef >-> AST.fundef.
+
+
+Definition globdef_of_globdef F V (gd: globdef (Ctypes.fundef F) V) : globdef (AST.fundef F) V :=
+  match gd with
+  | Gfun fd => Gfun (fundef_of_fundef fd)
+  | Gvar v => Gvar v
+  end.
+
+Section CSPECIFIC.
+
+  Definition is_external F (gd: globdef (Ctypes.fundef F) type): bool :=
+    match gd with
+    | Gfun fd => is_external_fd fd
+    | Gvar _ => false
+    end
+  .
+
+  Definition revive {F} (skenv: SkEnv.t) (prog: Ctypes.program F): Genv.t (Ctypes.fundef F) type :=
+    skenv.(Genv_map_defs) (fun blk gd => (do id <- skenv.(Genv.invert_symbol) blk;
+                                         do gd <- prog.(prog_defmap) ! id;
+                                         assertion (negb (is_external gd));
+                                         Some gd))
+  .
+
+  Lemma revive_no_external
+        F (prog: Ctypes.program F)
+        skenv blk gd
+        (DEF: Genv.find_def (revive skenv prog) blk = Some gd)
+        (EXTERNAL: is_external gd)
+    :
+      False
+  .
+  Proof.
+    unfold revive in *.
+    apply_all_once Genv_map_defs_def. des.
+    u in *. des_ifs.
+  Qed.
+  
+  Definition signature_of_function (f: function) :=
+    {| sig_args := map typ_of_type (map snd (fn_params f));
+       sig_res  := opttyp_of_type (fn_return f);
+       sig_cc   := fn_callconv f |}.
+  
+  Definition of_program {F} (get_sg: F -> signature) (prog: Ctypes.program F): Sk.t :=
+    mkprogram (skdefs_of_gdefs get_sg (map (update_snd (@globdef_of_globdef F type)) prog.(prog_defs))) prog.(prog_public) prog.(prog_main)
+  .
+
+  Lemma of_program_defs
+        F
+        get_sg
+        (p: Ctypes.program F)
+    :
+      (of_program get_sg p).(defs) = p.(defs)
+  .
+  Proof.
+    destruct p; ss.
+    Local Opaque in_dec.
+    u; ss.
+    Local Transparent in_dec.
+    apply Axioms.functional_extensionality. intro id; ss.
+    Check (in_dec ident_eq id (map fst prog_defs)).
+    rewrite map_map. rewrite map_map. ss.
+  Qed.
+
+End CSPECIFIC.
+
+
