cfrontend/CsemC.v
@@ -1,0 +1,225 @@
+Require Import CoqlibC Maps.
+Require Import ASTC Integers Values Events Memory Globalenvs.
+Require Import Op Registers.
+Require Import sflib.
+Require Import SmallstepC.
+(** newly added **)
+Require Export Simulation Csem Cop Ctypes Ctyping Csyntax Cexec.
+Require Import Skeleton Mod ModSem.
+Require Import AsmregsC CtypesC.
+Require Import Conventions.
+(* Require Import Locations. *)
+
+Set Implicit Arguments.
+
+
+
+
+
+Section CEXTRA.
+
+  Definition is_external (ge: genv) (s:state) : Prop:=
+    match s with
+    | Callstate fptr ty args k m  =>
+      match Genv.find_funct ge fptr with
+      | Some f =>
+        match f with
+        | External ef targs tres cconv => is_external_ef ef
+        | _ => False
+        end
+      | None => False
+      end
+    | _ => False
+    end
+  .
+
+  (* Variable ge_ge: Genv.t fundef type. *)
+  (* Variable ce_ge: composite_env. *)
+
+  (* Definition ge := Build_genv ge_ge ce_ge. *)
+  
+  (* Definition semantics_with_ge := Semantics_gen step bot1 final_state ge ge. *)
+
+  (* (* *************** ge is parameterized *******************) *)
+
+  (* Lemma semantics_receptive *)
+  (*       st *)
+  (*       (INTERNAL: ~ is_external ge st) *)
+  (*   : *)
+  (*     receptive_at semantics_with_ge st *)
+  (* . *)
+  (* Proof. *)
+  (*   admit "this should hold". *)
+  (* Qed. *)
+
+(*   Lemma semantics_determinate *)
+(*         st *)
+(*         (INTERNAL: ~is_external ge st) *)
+(*     : *)
+(*       determinate_at semantics_with_ge st *)
+(*   . *)
+(*   Proof. *)
+(*     admit "this should hold". *)
+(*   Qed. *)
+
+End CEXTRA.
+(*** !!!!!!!!!!!!!!! REMOVE ABOVE AFTER MERGING WITH MIXED SIM BRANCH !!!!!!!!!!!!!!!!!! ***)
+
+
+Definition get_mem (st: state): option mem :=
+  match st with
+  | State _ _ _ _ m0 => Some m0
+  | ExprState _ _ _ _ m0 => Some m0
+  | Callstate _ _ _ _ m0 => Some m0
+  | Returnstate _ _ m0 => Some m0
+  | Stuckstate => None
+  end
+.
+
+Section MODSEM.
+
+  Variable skenv_link: SkEnv.t.
+  Variable p: program.
+  (* Set Printing All. *)
+  Let skenv: SkEnv.t := skenv_link.(SkEnv.project) (defs p).
+  Let ce_ge: composite_env := prog_comp_env p.
+  Let ge_ge: Genv.t fundef type := revive skenv p.
+  Let ge: genv := Build_genv ge_ge ce_ge.
+
+  Inductive at_external (skenv_link: SkEnv.t): state -> Args.t -> Prop :=
+  | at_external_intro
+      fptr_arg tyf vs_arg sg_arg targs tres cconv k m0
+      (EXTERNAL: ge.(Genv.find_funct) fptr_arg = None)
+      (SIG: exists skd, skenv_link.(Genv.find_funct) fptr_arg = Some skd
+                   /\ SkEnv.get_sig skd = sg_arg
+                   /\ tyf = Tfunction targs tres cconv
+                   /\ signature_of_type targs tres cconv = sg_arg)                  
+    (* /\ type_of_fundef skd = tyf) *)
+    (* how can i check sg_args and tyf are same type? *)
+    (* typ_of_type function is a projection type to typ. it delete some info *)
+    :
+      at_external skenv_link (Callstate fptr_arg tyf vs_arg k m0)
+                  (Args.mk fptr_arg vs_arg m0)
+  .
+
+  Inductive initial_frame (args: Args.t)
+    : state -> Prop :=
+  | initial_frame_intro
+      fd k tyf
+      (FINDF: Genv.find_funct ge args.(Args.fptr) = Some (Internal fd))
+      (TYPE: type_of_fundef (Internal fd) = tyf)
+    :
+      initial_frame args
+                    (Callstate args.(Args.fptr) tyf args.(Args.vs) k args.(Args.m))
+  .
+
+  Inductive final_frame: state -> Retv.t -> Prop :=
+  | final_frame_intro
+      v_ret m_ret
+      (* (CONT: forall f e C ty k', k <> Kcall f e C ty k') *)
+    :
+      final_frame (Returnstate v_ret Kstop m_ret) (Retv.mk v_ret m_ret)
+  .
+
+  Inductive after_external: state -> Retv.t -> state -> Prop :=
+  | after_external_intro
+      fptr_arg tyf vs_arg m_arg
+      k retv
+    :
+      after_external (Callstate fptr_arg tyf vs_arg k m_arg)
+                     retv
+                     (Returnstate retv.(Retv.v) k retv.(Retv.m))
+  .
+
+  Program Definition modsem: ModSem.t :=
+    {|
+      ModSem.step := step;
+      ModSem.at_external := at_external;
+      ModSem.initial_frame := initial_frame;
+      ModSem.final_frame := final_frame;
+      ModSem.after_external := after_external;
+      ModSem.globalenv := ge;
+      ModSem.skenv := skenv; 
+    |}
+  .
+  Next Obligation. ii; ss; des. inv_all_once; ss; clarify. Qed.
+  Next Obligation. ii; ss; des. inv_all_once; ss; clarify. Qed.
+  Next Obligation. ii; ss; des. inv_all_once; ss; clarify. Qed.
+  Next Obligation. ii; ss; des. inv_all_once; ss; clarify. inv H.
+                   inv_all_once; ss; clarify. Qed.
+  Next Obligation. ii; ss; des. inv_all_once. inv H. inv H. Qed.
+                   (* specialize (CONT f e C ty k0). clarify. Qed. *)
+  Next Obligation. ii; ss; des. inv_all_once; ss; clarify. Qed.
+
+  Lemma not_external
+    :
+      is_external ge <1= bot1
+  .
+  Proof.
+    ii. hnf in PR. des_ifs.
+    subst_locals.
+    unfold Genv.find_funct, Genv.find_funct_ptr in *. des_ifs.
+    eapply revive_no_external; eauto.
+  Qed.
+
+  (* Lemma lift_receptive_at *)
+  (*       st *)
+  (*       (RECEP: receptive_at (semantics_with_ge ge) st) *)
+  (*   : *)
+  (*     receptive_at modsem st *)
+  (* . *)
+  (* Proof. *)
+  (*   inv RECEP. econs; eauto; ii; ss. exploit sr_receptive_at; eauto. *)
+  (*   eapply match_traces_preserved; try eassumption. ii; ss. *)
+  (* Qed. *)
+
+  (* Lemma modsem_receptive *)
+  (*       st *)
+  (*   : *)
+  (*     receptive_at modsem st *)
+  (* . *)
+  (* Proof. *)
+  (*   econs. i. *)
+  (*   eapply lift_receptive_at. eapply semantics_receptive. ii. eapply not_external; eauto. Qed. *)
+
+  (* not determ *)
+  (* Lemma lift_determinate_at *)
+  (*       st0 *)
+  (*       (DTM: determinate_at (semantics_with_ge ge) st0) *)
+  (*   : *)
+  (*     determinate_at modsem st0 *)
+  (* . *)
+  (* Proof. *)
+  (*   inv DTM. econs; eauto; ii; ss. *)
+  (*   determ_tac sd_determ_at. esplits; eauto. *)
+  (*   eapply match_traces_preserved; try eassumption. ii; ss. *)
+  (* Qed. *)
+
+  (* Lemma modsem_determinate *)
+  (*       st *)
+  (*   : *)
+  (*     determinate_at modsem st *)
+  (* . *)
+  (* Proof. eapply lift_determinate_at. eapply semantics_determinate. ii. eapply not_external; eauto. Qed. *)
+
+
+End MODSEM.
+
+Section MODULE.
+
+  Variable p: program.
+
+  Program Definition module: Mod.t :=
+    {|
+      Mod.data := p;
+      Mod.get_sk := of_program signature_of_function ;
+      Mod.get_modsem := modsem;
+    |}
+  .
+  Next Obligation.
+    rewrite CtypesC.of_program_defs.
+    eapply SkEnv.project_impl_spec; eauto.
+  Qed.
+
+End MODULE.
+
