cfrontend/UpperBound_B.v
@@ -1,0 +1,1215 @@
+Require Import CoqlibC Maps.
+Require Import ASTC Integers Floats Values MemoryC Events Globalenvs Smallstep.
+Require Import Locations Stacklayout Conventions Linking.
+(** newly added **)
+Require Export Csem Cop Ctypes Ctyping Csyntax Cexec.
+Require Import Simulation Memory ValuesC.
+Require Import Skeleton ModSem Mod sflib.
+Require Import CtypesC CsemC Sem Syntax LinkingC Program.
+
+Set Implicit Arguments.
+
+Local Opaque Z.mul.
+
+Section PRESERVATION.
+
+  Existing Instance Val.mi_final.
+
+(** PLAN B-0*)
+
+(*
+B-0
+* : Physical
++ : Logical 
+c0 * empty
+>=
+c0 + empty
+*)
+  
+ 
+  Section PLANB0.
+(** ********************* linking *********************************)  
+
+  (* Variable prog0: Csyntax.program. *)
+
+  (* Lemma empty_lemma *)
+  (*   : *)
+  (*     build_composite_env nil = Errors.OK (PTree.empty composite). *)
+  (* Proof. auto. Qed. *)
+  
+  (* Let empty_prog : Csyntax.program := *)
+  (*   Build_program nil nil prog0.(prog_main) nil empty_lemma. *)
+
+  Variable prog: Csyntax.program.
+  (* Hypothesis LINK : link prog0 empty_prog = Some prog. *)
+  Let tprog : Syntax.program := List.map CsemC.module [prog].
+  
+  (* TODO: prog always exists *)
+
+(** ********************* genv *********************************)
+
+  Variable sk_tgt: Sk.t.
+  Hypothesis LINK_SK_TGT: link_sk tprog = Some sk_tgt.
+  (* TODO: consider linking fail case *)
+  Let skenv_link := Sk.load_skenv sk_tgt.
+
+  Let ge := globalenv prog.
+  Let tge_ce : composite_env := prog_comp_env prog.
+  Let tge := load_genv tprog skenv_link.
+
+  Inductive match_states : Csem.state -> Sem.state -> nat -> Prop :=
+  | match_states_intro
+      fr frs (st: Csem.state)
+      (FRAME: fr = Frame.mk (CsemC.modsem skenv_link prog) st)
+    :
+      match_states st (Sem.State (fr::frs)) 0
+  .  
+  (* | match_states_internal_stmt *)
+  (*     fr frs p f s k e m n *)
+  (*     (FRAME: fr = Frame.mk (CsemC.modsem skenv_link p) *)
+  (*                           (Csem.State f s k e m)) *)
+  (*   : *)
+  (*     match_states (Csem.State f s k e m) (Sem.State (fr::frs)) n *)
+  (* | match_states_internal_expr *)
+  (*     fr frs p f ex k e m n *)
+  (*     (FRAME: fr = Frame.mk (CsemC.modsem skenv_link p) *)
+  (*                           (Csem.ExprState f ex k e m)) *)
+  (*   : *)
+  (*     match_states (Csem.ExprState f ex k e m) (Sem.State (fr::frs)) n *)
+  (* . *)
+  
+      
+  (* | match_states_external *)
+  (* | match_states_ *)
+  
+  
+  Definition local_genv (p : Csyntax.program) :=
+    (skenv_link.(SkEnv.project) p.(defs)).(revive) p.
+
+  (* Inductive genv_le (j: meminj) (src_ge tgt_ge: Genv.t fundef unit): Prop := *)
+  (* | genv_le_intro  *)
+  (*     (SYMB: forall id b (FIND: Genv.find_symbol src_ge id = Some b), *)
+  (*         Genv.find_symbol tgt_ge id = Some b *)
+  (*         /\ j b = Some (b, 0)) (* is it needed? *) *)
+  (*     (DEFS: forall b0 d (FIND: Genv.find_def src_ge b0 = Some d), *)
+  (*         exists b1, j b0 = Some (b1, 0) *)
+  (*                    /\ Genv.find_def tgt_ge b1 = Some d). *)
+
+  (* Lemma genv_le_incr j0 j1 src_ge tgt_ge *)
+  (*       (INCR: inject_incr j0 j1) *)
+  (*       (GENVLE: genv_le j0 src_ge tgt_ge) *)
+  (*   :       *)
+  (*      genv_le j1 src_ge tgt_ge. *)
+  (* Proof. *)
+  (*   inv GENVLE. econs; ii; ss. *)
+  (*   - specialize (SYMB _ _ FIND). des. eauto. *)
+  (*   - specialize (DEFS _ _ FIND). des. esplits; eauto. *)
+  (* Qed. *)
+
+
+
+(** ********************* transf step  *********************************)
+
+  Lemma match_state_xsim
+    :
+      forall st_src st_tgt (MTCHST: match_states st_src st_tgt 0),
+        xsim (Csem.semantics prog) (Sem.sem tprog) lt 0%nat st_src st_tgt.
+  Proof.
+    pcofix CIH. i. pfold.
+    inv MTCHST.
+    destruct st_src.
+    - (* State *)
+      right. econs.
+      + i. inv FINALTGT. inv FINAL.
+      + i. econs. i. inv STEPTGT; try (by (ss; des_ifs)).
+        * ss. des_ifs. inv AT.
+        * ss. inv STEP; ss.
+          { inv H. }
+          exists 0%nat, st0.
+          split.
+          ** left. apply plus_one. econs 2.
+             inv H; try (by econs).
+          ** right. eapply CIH.
+             econs; eauto.
+        * inv FINAL.
+      + i.
+        specialize (SAFESRC _ (star_refl _ _ _)). inv SAFESRC.
+        * des. inv H.
+        * right. des.
+          exists t. des_ifs. ss. eexists. econs. ss.
+          inv H. inv H0.
+          right. inv H0; try (by econs).
+    - (* ExprState *)
+      right. econs.
+      + i. inv FINALTGT. inv FINAL.
+      + i. econs. i. inv STEPTGT; try (by (ss; des_ifs)).
+        * ss. des_ifs. inv AT.
+        * ss. inv STEP; ss.
+          ** exists 0%nat, st0.
+             split; cycle 1.
+             { right. eapply CIH.
+               econs; eauto. }
+             { left. apply plus_one. econs 1.
+               inv H; try (econs; eauto).
+               - admit "".
+               - admit "".
+               - admit "". }
+          ** exists 0%nat, st0.
+             split; cycle 1.
+             { right. eapply CIH.
+               econs; eauto. }
+             { left. apply plus_one. econs 2.
+               inv H; try (by econs). }
+        * inv FINAL.
+      + i.
+        specialize (SAFESRC _ (star_refl _ _ _)). des.
+        * left. inv SAFESRC.
+        * right.
+          inv SAFESRC.
+          ** inv H.
+             { exploit step_internal; eauto; ss. econs 1. econs; eauto. admit "". }
+             { exploit step_internal; eauto; ss. econs 1. econs 2; eauto. admit "". }
+             { exploit step_internal; eauto; ss. econs 1. econs 3; eauto. }
+             { exploit step_internal; eauto; ss. econs 1. econs 4; eauto. admit "". }
+          ** inv H; exploit step_internal; eauto; ss; try (by econs 2; econs; eauto).
+    - (* Callstate *)
+      right. econs.
+      + i. inv FINALTGT. inv FINAL.
+      + i. econs. i. inv STEPTGT.
+        * ss. inv AT. inv EXTERNAL. des.
+          admit " by SIG && H0".
+        * ss. inv STEP; ss.
+          { inv H. }
+          exists 0%nat, st0.
+          split.
+          ** left. apply plus_one. econs 2.
+             inv H; try (by econs).
+             { admit "". }
+             { ss. econs; admit "". }
+          ** right. eapply CIH.
+             econs; eauto.
+        * inv FINAL.
+      + i.
+        specialize (SAFESRC _ (star_refl _ _ _)). des.
+        * left. inv SAFESRC.
+        * right.
+          inv SAFESRC.
+          { inv H. }
+          exists t. eexists. econs. ss.
+          inv H; econs 2; ss.
+          { admit "prove it". }
+          { admit "prove it". }
+    - (* Returnstate *)
+      (* right. econs. *)
+      (* + i. inv FINALTGT. inv FINAL. ss. esplits. *)
+      (*   * econs. *)
+      (*   * rewrite INT. econs. *)
+      (* + i. econs. i. inv STEPTGT; ss. *)
+      (*   * inv AT. *)
+      (*   * inv STEP. *)
+      (*     { inv H. } *)
+      (*     exists 0%nat, st0. *)
+      (*     split. *)
+      (*     ** left. apply plus_one. econs 2. *)
+      (*        inv H; econs. *)
+      (*     ** right. eapply CIH. *)
+      (*        econs; eauto. *)
+      (*   * admit "final frame strange". *)
+      (* + i. *)
+      (*   specialize (SAFESRC _ (star_refl _ _ _)). des. *)
+      (*   * admi *)
+      (*   * right. *)
+      (*     inv SAFESRC. *)
+      (*     { inv H. } *)
+      (*     exists t. eexists. econs. ss. *)
+      (*     inv H; econs 2; ss. *)
+      (*     { admit "prove it". } *)
+      (*     { admit "prove it". } *)
+      admit "final frame strange".
+    - (* Stuckstate *)
+      right. econs.
+      + i. inv FINALTGT. inv FINAL.
+      + i. econs. i. inv STEPTGT; try (by (ss; des_ifs)).
+        * ss. des_ifs. inv AT.
+        * ss. inv STEP; ss; inv H.
+        * inv FINAL.
+      + i.
+        specialize (SAFESRC _ (star_refl _ _ _)). inv SAFESRC.
+        * des. inv H.
+        * right. des; inv H; inv H0.
+      Unshelve.
+      auto. auto. auto. auto. auto. auto. auto. auto. auto. auto.
+  Qed.
+
+  Lemma transf_xsim_properties
+    :
+        xsim_properties (Csem.semantics prog) (Sem.sem tprog) nat lt.
+  Proof.
+    admit "prove it".
+  Qed.
+
+  Lemma transf_program_correct:
+    mixed_simulation (Csem.semantics prog) (Sem.sem tprog).
+  Proof.
+    eapply Mixed_simulation. eapply transf_xsim_properties.
+  Qed.
+
+
+  End PLANB0.
+(** ********************* initial memory *********************************)
+  
+  Variable m_init : mem.
+  Hypothesis INIT_MEM: sk.(Sk.load_mem) = Some m_init.
+  (* TODO: m_init exist *)
+
+  Definition m_tgt_init := m_init.
+  (* Variable m_tgt_init : mem. *)
+  (* Hypothesis INIT_TGT_MEM: Genv.init_mem tprog = Some m_tgt_init. *)
+  Lemma TGT_INIT_MEM: Genv.init_mem tprog = Some m_tgt_init.
+  Proof.
+    unfold Sk.load_mem in *.
+    eapply Genv.init_mem_match
+      with (ctx := tt) (match_fundef := top3) (match_varinfo := top2);
+      [| eapply INIT_MEM]. econs.
+    - admit "list_forall2 (match_ident_globdef top3 top2 ()) (prog_defs sk) (prog_defs tprog)".
+    - admit "prog_main tprog = prog_main sk /\ prog_public tprog = prog_public sk".
+  Qed.
+
+  Definition init_inject := Mem.flat_inj (Mem.nextblock m_init).
+
+  Lemma initmem_inject: Mem.inject init_inject m_init m_tgt_init.
+  Proof.
+    eapply Genv.initmem_inject. unfold Sk.load_mem in INIT_MEM. eauto.
+  Qed.
+
+  Lemma init_inject_genv_le p: genv_le init_inject (local_genv p) tge.
+  Admitted.
+
+  Lemma local_genv_le j p
+        (INCR: inject_incr init_inject j)
+    : genv_le j (local_genv p) tge.
+  Proof.
+    eapply genv_le_incr; eauto. apply init_inject_genv_le.
+  Qed.  
+
+  Lemma ALLOC_NEXT_INCR F V (gen: Genv.t F V) x m0 m1
+        (ALLOC: Genv.alloc_global gen m0 x = Some m1)
+    :
+      Plt (Mem.nextblock m0) (Mem.nextblock m1).
+  Proof.
+    destruct x. ss. destruct g; des_ifs.
+    - apply Mem.nextblock_alloc in Heq.
+      eapply Mem.nextblock_drop in ALLOC.
+      rewrite ALLOC. rewrite Heq. apply Plt_succ.
+    - apply Mem.nextblock_alloc in Heq.
+      apply Genv.store_zeros_nextblock in Heq0.
+      apply Genv.store_init_data_list_nextblock in Heq1.
+      eapply Mem.nextblock_drop in ALLOC.
+      rewrite ALLOC. rewrite Heq1. rewrite Heq0. rewrite Heq.
+      apply Plt_succ.
+  Qed.
+
+  Lemma ALLOCS_NEXT_INCR F V (gen: Genv.t F V) l m0 m1
+        (ALLOC: Genv.alloc_globals gen m0 l = Some m1)
+    :
+      Ple (Mem.nextblock m0) (Mem.nextblock m1).
+  Proof.
+    revert l gen m0 m1 ALLOC. induction l; i; ss; clarify.
+    - reflexivity.
+    - des_ifs. etrans.
+      + apply Plt_Ple. eapply ALLOC_NEXT_INCR; eauto.
+      + eapply IHl; eauto.
+  Qed.
+
+  Lemma init_mem_nextblock F V (p: AST.program F V) m
+        (INIT: Genv.init_mem p = Some m)
+    :
+      Plt 1 (Mem.nextblock m).
+  Proof.
+    unfold Genv.init_mem in *.
+    eapply ALLOCS_NEXT_INCR in INIT.
+    ss. apply Pos.le_succ_l. ss.
+  Qed.
+  
+(** ********************* regset *********************************)
+
+  Definition initial_regset : regset := 
+    (Pregmap.init Vundef)
+      # PC <- (Genv.symbol_address tge tprog.(prog_main) Ptrofs.zero)
+      # RA <- Vnullptr
+      # RSP <- (Vptr 1%positive Ptrofs.zero true).
+
+  Definition initial_tgt_regset := initial_regset.
+
+  Definition agree (j: meminj) (rs_src rs_tgt: regset) : Prop :=
+    forall pr, Val.inject j (rs_src pr) (rs_tgt pr).
+
+  Lemma update_agree j rs_src rs_tgt pr v
+        (AGREE: agree j rs_src rs_tgt)
+        (UPDATE: Val.inject j v (rs_tgt # pr))
+    :
+      agree j (rs_src # pr <- v) rs_tgt.
+  Proof.
+    destruct pr; intros pr0; specialize (AGREE pr0); destruct pr0; eauto.
+    - destruct i, i0; eauto.
+    - destruct f, f0; eauto.
+    - destruct c, c0; eauto.
+  Qed.
+
+  Lemma update_agree2 j rs_src rs_tgt pr v_src v_tgt
+        (AGREE: agree j rs_src rs_tgt)
+        (UPDATE: Val.inject j v_src v_tgt)
+    :
+      agree j (rs_src # pr <- v_src) (rs_tgt # pr <- v_tgt).
+  Proof.
+    destruct pr; intros pr0; specialize (AGREE pr0); destruct pr0; eauto.
+    - destruct i, i0; eauto.
+    - destruct f, f0; eauto.
+    - destruct c, c0; eauto.
+  Qed.
+
+  Lemma initial_regset_agree: agree init_inject initial_regset initial_tgt_regset.
+  Proof.
+    unfold initial_tgt_regset, initial_regset.
+    repeat eapply update_agree2; ss; eauto.
+    - unfold Genv.symbol_address; des_ifs. econs; eauto.
+      unfold init_inject, Mem.flat_inj. des_ifs.
+      exfalso. eapply Genv.genv_symb_range in Heq. 
+      unfold tge in *. erewrite Genv.init_mem_genv_next in Heq. eauto.
+      apply TGT_INIT_MEM. symmetry. apply Ptrofs.add_zero.
+    - econs.
+    - econs.
+      + unfold init_inject, Mem.flat_inj; des_ifs.
+        exfalso. apply n. eapply init_mem_nextblock.
+        unfold Sk.load_mem in INIT_MEM. apply INIT_MEM.
+      + symmetry. apply Ptrofs.add_zero.
+  Qed.      
+
+  Inductive inj_same (j: meminj) v_caller v_callee : Prop :=
+  | inj_same_intro
+      blk_caller blk_callee blk delta delta' ofs
+      (CALLERRSP: v_caller = Vptr blk_caller ofs true)
+      (CALLEERSP: v_callee = Vptr blk_callee Ptrofs.zero true)
+      (EQ: Ptrofs.repr delta' = ofs)
+      (CALLER: j blk_caller = Some (blk, delta))
+      (CALLEE: j blk_callee = Some (blk, delta + delta')).
+
+  Lemma inj_same_inj j v_caller v_callee v_tgt
+        (SAME: inj_same j v_caller v_callee)
+        (INJ: Val.inject j v_caller v_tgt)
+    :
+      Val.inject j v_callee v_tgt.
+  Proof.
+    inv SAME. inv INJ. clarify. econs; eauto. 
+    rewrite Ptrofs.add_zero_l.
+    rewrite IntegersC.Ptrofs_add_repr.
+    f_equal. apply Z.add_comm.
+  Qed.
+
+  Lemma inj_same_inj2 j v_caller v_callee v_tgt
+        (SAME: inj_same j v_caller v_callee)
+        (INJ: Val.inject j v_callee v_tgt)
+    :
+      Val.inject j v_caller v_tgt.
+  Proof.
+    inv SAME. inv INJ. clarify. econs; eauto. 
+    rewrite Ptrofs.add_zero_l.
+    rewrite IntegersC.Ptrofs_add_repr.
+    f_equal. apply Z.add_comm.
+  Qed.
+
+  Definition to_fake (v: val) : val :=
+    match v with
+    | Vptr blk ofs true => Vptr blk ofs false
+    | _ => v
+    end.
+
+  Lemma to_fake_inj j v_src v_tgt
+        (INJ: Val.inject j v_src v_tgt)
+    :
+        Val.inject j (to_fake v_src) v_tgt.
+  Proof. unfold to_fake. inv INJ; econs; eauto. Qed.
+
+  Definition extcall_args_reg (mr: mreg) (sg: signature):
+    {In (R mr) (regs_of_rpairs (loc_arguments sg))} +
+    {~ In (R mr) (regs_of_rpairs (loc_arguments sg))}.
+  Proof.
+    generalize (regs_of_rpairs (loc_arguments sg)). induction l.
+    - ss. tauto.
+    - ss. inv IHl; [tauto|].
+      destruct a.
+      + destruct (mreg_eq r mr); [clarify; eauto|].
+        right. intros []; clarify.
+      + right. intros []; clarify.
+  Qed.
+
+  Lemma extcall_args_callee_save_disjoint sg mr
+        (EXT: In (R mr) (regs_of_rpairs (loc_arguments sg)))
+    :
+      ~ Conventions1.is_callee_save mr.
+  Proof.
+    destruct sg. ss.
+    unfold loc_arguments in *.
+    ss. replace Archi.ptr64 with true in *; eauto.
+    assert (forall l mr p q r,
+                In (R mr) (regs_of_rpairs (loc_arguments_64 l p q r)) ->
+                ~ is_callee_save mr); eauto.
+    induction l; ss; i; destruct a; des_ifs; ss; des; eauto; inv H; ss.
+  Qed.
+
+  Definition src_init_rs sg (rs_src: regset) (rsp: val) : regset :=
+    fun (pr : PregEq.t) =>
+      match Asm.to_mreg pr with
+      | Some mr =>
+        if (extcall_args_reg mr sg)
+        then (rs_src pr)
+        else (to_fake (rs_src pr))
+      | None =>
+        match pr with
+        | IR RSP => rsp
+        | PC => rs_src PC
+        | RA => rs_src RA
+        | _ => to_fake (rs_src pr)
+        end
+      end.
+
+  Definition callee_injection (j: meminj) old_blk new_blk old_delta : meminj :=
+    fun blk => if (eq_block blk new_blk)
+               then
+                 (match (j old_blk) with
+                  | None => None
+                  | Some (blk', delta) => Some (blk', old_delta + delta)
+                  end)
+               else (j blk).
+
+  Lemma src_init_rs_agree' j sg rsp (rs_src rs_tgt: regset)
+        (AGREE: agree j rs_src rs_tgt)
+        (RSPINJ: Val.inject j rsp (rs_tgt # RSP))
+    :
+      agree j (src_init_rs sg rs_src rsp) rs_tgt.
+  Proof.
+    intros pr. specialize (AGREE pr). unfold src_init_rs.
+    destruct pr; ss; try (destruct (extcall_args_reg _ sg); ss; eapply to_fake_inj; eauto).
+    - destruct i; try (destruct (extcall_args_reg _ sg); ss; eapply to_fake_inj; eauto); ss.
+    - destruct f; try (destruct (extcall_args_reg _ sg); ss; eapply to_fake_inj; eauto); ss.
+    - eapply to_fake_inj; eauto.
+  Qed.
+
+  Lemma src_init_rs_agree j sg blk delta ofs new_blk (rs_src rs_tgt: regset)
+        (RSPPTR: rs_src # RSP = Vptr blk ofs true)
+        (DELTA: Ptrofs.repr delta = ofs)
+        (INJNONE: j new_blk = None)
+        (AGREE: agree j rs_src rs_tgt)
+    :
+      agree (callee_injection j blk new_blk delta)
+            (src_init_rs sg rs_src (Vptr new_blk Ptrofs.zero true)) rs_tgt.
+  Proof.
+    set (RSPAGREE := AGREE RSP).
+    rewrite RSPPTR in *. inv RSPAGREE. eapply src_init_rs_agree'.
+    - intros pr. specialize (AGREE pr).
+      inv AGREE; econs; clarify; eauto; unfold callee_injection; des_ifs.
+    - unfold callee_injection. rewrite <- H1. econs. des_ifs.
+      rewrite IntegersC.Ptrofs_add_repr. rewrite Ptrofs.add_zero_l. auto.
+  Qed.
+
+  Inductive almost_eq : val -> val -> Prop :=
+  | almost_eq_refl v : almost_eq v v
+  | almost_eq_ptr blk ofs b1 b2 : almost_eq (Vptr blk ofs b1) (Vptr blk ofs b2)
+  .
+
+  Lemma to_fake_almost_eq v
+    :
+      almost_eq v (to_fake v).
+  Proof.
+    destruct v; try econs. destruct b0; econs.
+  Qed.
+
+  Lemma almost_eq_commute j v_src0 v_src1 v_tgt
+        (INJ: Val.inject j v_src1 v_tgt)
+        (EQ: almost_eq v_src0 v_src1)
+    :
+      Val.inject j v_src0 v_tgt.
+  Proof.
+    inv EQ; eauto.
+    destruct b1, b2; inv INJ; try econs; eauto. clarify.
+  Qed.
+
+  Lemma lessdef_commute j v_src0 v_src1 v_tgt
+        (INJ: Val.inject j v_src1 v_tgt)
+        (LESS: Val.lessdef v_src0 v_src1)
+    :
+      Val.inject j v_src0 v_tgt.
+  Proof.
+    inv LESS; inv INJ; eauto.
+  Qed.
+
+  Inductive wf_init_rs (j: meminj) (rs_caller rs_callee: regset) : Prop :=
+  | wf_init_rs_intro
+      (PCSAME: rs_caller # PC = rs_callee # PC)
+      (RASAME: rs_caller # RA = rs_callee # RA)
+      (RSPSAME: inj_same j (rs_caller # RSP) (rs_callee # RSP))
+      (CALLEESAVE: forall mr, Conventions1.is_callee_save mr ->
+                              almost_eq (rs_caller (to_preg mr))
+                                        (rs_callee (to_preg mr)))
+  .    
+
+  Lemma src_init_rs_wf j old_blk new_blk ofs (rs: regset) sg b' delta
+        (INJ_NONE: j new_blk = None)
+        (INJ_SOME: j old_blk = Some (b', delta))
+        (RSRSP: rs # RSP = Vptr old_blk ofs true)
+    :
+      wf_init_rs
+      (callee_injection j old_blk new_blk (Ptrofs.unsigned ofs))
+      rs
+      (src_init_rs sg rs (Vptr new_blk Ptrofs.zero true)).
+  Proof.
+    econs; ss.
+    - econs; eauto; ss.
+      + apply Ptrofs.repr_unsigned.
+      + unfold callee_injection. des_ifs. apply INJ_SOME.
+      + unfold callee_injection. des_ifs.
+        rewrite Z.add_comm. auto.
+    - intros. unfold src_init_rs. Opaque to_fake.
+      destruct mr; ss; clarify; des_ifs; try econs; try apply to_fake_almost_eq.
+  Qed.          
+
+(** ********************* match stack *********************************)
+  
+  Inductive match_stack (j: meminj) : regset -> list Frame.t -> Prop :=
+  | match_stack_init
+      init_rs
+      (RSRA: init_rs # RA = Vnullptr)
+      (RSPC: init_rs # PC = Genv.symbol_address tge tprog.(prog_main) Ptrofs.zero)
+      (SIG: skenv_link.(Genv.find_funct) (Genv.symbol_address tge tprog.(prog_main) Ptrofs.zero) = Some (Internal signature_main))
+    :
+      match_stack j init_rs nil
+  | match_stack_cons
+      fr frs p st b init_rs0 init_rs1
+      (FRAME: fr = Frame.mk (AsmC.modsem skenv_link p) (AsmC.mkstate init_rs1 st b))
+      (STACK: match_stack j init_rs1 frs)
+      (WF: wf_init_rs j st.(st_rs) init_rs0)
+    :
+      match_stack j init_rs0 (fr::frs)
+  .
+
+  Inductive match_stack_call (j: meminj) : mem -> regset -> list Frame.t -> Prop :=
+  | match_stack_call_init
+      init_rs m
+      (MEM: m = m_init)
+      (INITRS: init_rs = initial_regset)
+    :
+      match_stack_call j m init_rs nil
+  | match_stack_call_cons
+      fr frs p st b init_rs0 init_rs1 m
+      (FRAME: fr = Frame.mk (AsmC.modsem skenv_link p)
+                            (AsmC.mkstate init_rs1 st b))
+      (INITRS: init_rs0 = st.(st_rs))
+      (STACK: match_stack j init_rs1 frs)
+      (MEM: m = st.(st_m))      
+    :
+      match_stack_call j m init_rs0 (fr::frs)
+  .
+
+  Lemma match_stack_incr j1 j2 init_rs l
+        (INCR: inject_incr j1 j2)
+        (MATCH: match_stack j1 init_rs l)
+    :
+      match_stack j2 init_rs l.
+  Proof.
+    revert init_rs INCR MATCH. induction l; ss; ii; inv MATCH; econs; ss; eauto.
+    inv WF. econs; eauto.
+    inv RSPSAME. econs; eauto.
+  Qed.
+
+  Lemma frame_inj a0 b0 a1 b1
+        (EQ: Frame.mk a0 b0 = Frame.mk a1 b1)
+    : b0 ~= b1.
+  Proof. inv EQ. eauto. Qed.
+
+  Lemma asm_frame_inj se1 se2 p1 p2 st1 st2
+        (EQ : Frame.mk (modsem se1 p1) st1 = Frame.mk (modsem se2 p2) st2)
+    :
+      st1 = st2.
+  Proof. apply frame_inj in EQ. apply JMeq_eq. eauto. Qed.
+
+  Definition memcpy (m: mem) (blk: Values.block) (lo size: Z) : mem. Admitted.
+  
+  Lemma memcpy_spec1 m blk lo size
+    :
+      Mem.nextblock (memcpy m blk lo size) = Pos.succ m.(Mem.nextblock).
+  Admitted.
+
+  (* Lemma memcpy_spec2_1 m chunk blk lo size ofs *)
+  (*       (BOUND: 0 <= ofs < size) *)
+  (*   : *)
+  (*     Mem.load chunk (memcpy m blk lo size) (Mem.nextblock m) ofs = *)
+  (*     Mem.load chunk m blk (lo + ofs). *)
+  (* Admitted. *)
+
+  Lemma memcpy_spec2_2 m blk lo size blk0 ofs
+        (NEQ0: blk0 <> blk)
+        (NEQ1: blk0 <> m.(Mem.nextblock))
+    :
+      ZMap.get ofs (Mem.mem_contents (memcpy m blk lo size)) !! blk0 =
+      ZMap.get ofs (Mem.mem_contents m) !! blk0.
+  Admitted.
+
+  Lemma memcpy_load m chunk blk lo size ofs
+        (BOUND: 0 <= ofs < size)
+    :
+      Mem.load chunk (memcpy m blk lo size) (Mem.nextblock m) ofs =
+      Mem.load chunk m blk (lo + ofs).
+  Admitted.
+
+  Lemma memcpy_spec3_1 m blk lo size ofs k p
+        (BOUND: 0 <= ofs < size)
+    :
+      Mem.perm (memcpy m blk lo size) m.(Mem.nextblock) ofs k p <->
+      Mem.perm m blk (lo + ofs) k p.
+  Admitted.
+
+  Lemma memcpy_spec3_2 m blk lo size ofs k p
+        (BOUND: ~ 0 <= ofs < size)
+    :
+      ~ Mem.perm (memcpy m blk lo size) m.(Mem.nextblock) ofs k p.
+  Admitted.
+
+  Lemma memcpy_spec3_3 m blk lo size blk0 ofs k p
+        (NEQ0: blk0 <> blk)
+        (NEQ1: blk0 <> m.(Mem.nextblock))
+    :
+      Mem.perm (memcpy m blk lo size) blk0 ofs k p <->
+      Mem.perm m blk0 ofs k p.
+  Admitted.
+    
+  Lemma memcpy_spec3_4 m blk lo size ofs k p
+        (BOUND: 0 <= ofs < size)
+    :
+      ~ Mem.perm (memcpy m blk lo size) blk (lo + ofs) k p.
+  Admitted.
+
+  Lemma memcpy_spec3_5 m blk lo size ofs k p
+        (BOUND: ~ 0 <= ofs < size)
+    :
+      Mem.perm (memcpy m blk lo size) blk (lo + ofs) k p <->
+      Mem.perm m blk (lo + ofs) k p.
+  Admitted.
+
+  Lemma unfree_free_inj j (m_src0 m_src1 m_src2 m_tgt: mem) blk0 blk1 delta1 delta2 ofs1 ofs2 size
+        (DELTA1: Ptrofs.repr delta1 = ofs1)
+        (DELTA2: Ptrofs.repr delta2 = ofs2)
+        (FREE: Mem.free m_src0 blk0 delta1 (delta1 + size) = Some m_src1)
+        (UNFREE: Mem_unfree m_src1 blk1 delta2 (delta2 + 4 * size) = Some m_src2)
+        (SAME: inj_same j (Vptr blk1 ofs2 true) (Vptr blk0 ofs1 true))
+        (INJ: Mem.inject j m_src0 m_tgt)
+    :
+      Mem.inject j m_src2 m_tgt.
+  Admitted.
+
+  Lemma preg_case pr :
+    (exists mr, pr = to_preg mr) \/
+    (pr = PC) \/ (exists c, pr = CR c) \/ (pr = RSP) \/ (pr = RA)
+  .
+  Proof.
+    destruct (to_mreg pr) eqn:EQ.
+    - left. exists m. unfold to_mreg in *.
+      destruct pr; clarify.
+      destruct i; clarify; auto.
+      destruct f; clarify; auto.
+    - right. unfold to_mreg in *.
+      destruct pr; clarify; eauto.
+      destruct i; clarify; auto.
+      destruct f; clarify; auto.
+  Qed.
+
+  Lemma callee_save_agree j rs_caller init_rs rs_callee rs_tgt sg mr rs
+        (WF: wf_init_rs j rs_caller init_rs)
+        (AGREE: agree j rs_callee rs_tgt)
+        (INITSIG: exists skd, skenv_link.(Genv.find_funct) (init_rs # PC) = Some skd /\ SkEnv.get_sig skd = sg)
+        (RETV: loc_result sg = One mr)
+        (CALLEESAVE: forall mr, Conventions1.is_callee_save mr ->
+                                Val.lessdef (init_rs mr.(to_preg)) (rs_callee mr.(to_preg)))
+        (RSRA: rs_callee # PC = init_rs # RA)
+        (RSRSP: rs_callee # RSP = init_rs # RSP)
+        (RS: rs = (set_pair (loc_external_result sg) (rs_callee mr.(to_preg)) (Asm.regset_after_external rs_caller)))
+    :
+        agree j rs rs_tgt.
+  Proof.
+    inv WF. clarify.
+    - unfold loc_external_result. rewrite RETV. ss.
+      eapply update_agree; eauto.
+      unfold Asm.regset_after_external in *. intros pr. specialize (AGREE pr).
+      destruct (preg_case pr); des; clarify; ss.
+      + rewrite to_preg_to_mreg. des_ifs.
+        specialize (CALLEESAVE mr0). specialize (CALLEESAVE0 mr0).
+        rewrite Heq in *.
+        eapply almost_eq_commute with (v_src1 := init_rs (to_preg mr0)); eauto.
+        eapply lessdef_commute with (v_src1 := rs_callee (to_preg mr0)); eauto.
+      + rewrite RSRSP in *.
+        eapply inj_same_inj2; eauto.
+  Qed.
+
+  Inductive match_states : Sem.state -> Asm.state -> nat -> Prop :=
+  | match_states_intro
+      j fr frs p init_rs b rs_src rs_tgt m_src m_tgt n
+      (AGREE: agree j rs_src rs_tgt)
+      (INJ: Mem.inject j m_src m_tgt)
+      (INITINCR: inject_incr init_inject j)
+      (FRAME: fr = Frame.mk (AsmC.modsem skenv_link p)
+                            (AsmC.mkstate init_rs (Asm.State rs_src m_src) b))
+      (STACK: match_stack j init_rs frs)
+      (ORD: n = if (external_state skenv_link p (rs_src # PC))
+                then (length frs + 2)%nat else 0%nat)
+    :
+      match_states (State (fr::frs)) (Asm.State rs_tgt m_tgt) n
+  | match_states_call
+      j init_rs frs args m_src rs_tgt m_tgt ofs blk sg n
+      (STACK: match_stack_call j m_src init_rs frs)
+      (AGREE: agree j init_rs rs_tgt)
+      (INJECT: Mem.inject j m_src m_tgt)
+      (INITINCR: inject_incr init_inject j)
+      (FPTR: args.(Args.fptr) = init_rs # PC)
+      (SIG: exists skd, skenv_link.(Genv.find_funct) args.(Args.fptr)
+                        = Some skd /\ SkEnv.get_sig skd = sg)
+      (ARGS: extcall_arguments init_rs m_src sg args.(Args.vs))
+      (RSPPTR: init_rs # RSP = Vptr blk ofs true)
+      (FREE: Mem.free m_src blk ofs.(Ptrofs.unsigned) (ofs.(Ptrofs.unsigned) + 4 * (size_arguments sg)) = Some args.(Args.m))
+      (ORD: n = 1%nat)
+    :
+      match_states (Callstate args frs) (Asm.State rs_tgt m_tgt) n.
+
+  Lemma mem_free_none m blk lo hi
+        (EQ: lo = hi)
+    :
+      Mem.free m blk lo hi = Some m.
+  Proof. admit "mem_free_none". Qed.
+
+  Lemma symb_main :
+    Genv.find_symbol skenv_link (prog_main sk) =
+    Genv.find_symbol tge (prog_main tprog).
+  Proof. admit "". Qed.
+
+  Lemma transf_initial_states:
+    forall st1, Sem.initial_state prog st1 ->
+                exists st2, Asm.initial_state tprog st2 /\ match_states st1 st2 1.
+  Proof.
+    generalize TGT_INIT_MEM.
+    generalize initial_regset_agree.
+    generalize initmem_inject.
+    intros initmem_inject initial_regset_agree TGT_INT_MEM.
+    intros st1 INIT. inv INIT; clarify. esplits.
+    - econs; eauto.
+    - econs; ss; eauto; ss.
+      + econs; ss; eauto.
+      + unfold initial_regset.
+        rewrite Pregmap.gso; clarify.
+        rewrite Pregmap.gso; clarify. ss.
+        rewrite Pregmap.gss. unfold tge.
+        set (MAIN:= symb_main).
+        unfold Genv.symbol_address. unfold skenv_link, tge in *. rewrite MAIN. auto.
+      + econs.
+      + apply mem_free_none. ss.
+  Qed.
+
+  Lemma transf_final_states:
+    forall st1 st2 r n,
+      match_states st1 st2 n -> Sem.final_state st1 r -> Asm.final_state st2 r.
+  Proof.
+    intros st_src st_tgt r n MTCHST FINAL. inv FINAL. inv MTCHST. ss.
+    inv FINAL0. clarify. inv STACK. econs.
+    - specialize (AGREE PC). rewrite RSRA in *. rewrite RSRA0 in *.
+      inv AGREE; ss.
+    - des. rewrite RSPC in *. rewrite SIG in *. clarify.
+      ss. unfold signature_main, loc_arguments, loc_result in *.
+      Transparent Archi.ptr64. ss. unfold loc_result_64 in *. ss. clarify.
+      ss. specialize (AGREE RAX). rewrite INT in *. inv AGREE; auto.
+  Qed.  
+
+  Lemma step_return_simulation
+        fr0 fr1 frs retv st0 st_tgt n0
+        (FINAL: fr0.(Frame.ms).(ModSem.final_frame) fr0.(Frame.st) retv)
+        (AFTER: fr1.(Frame.ms).(ModSem.after_external) fr1.(Frame.st) retv st0)
+        (MTCHST: match_states (State (fr0 :: fr1 :: frs)) st_tgt n0)
+    :
+      exists n1, match_states (State ((fr1.(Frame.update_st) st0) :: frs)) st_tgt n1
+                 /\ (n1 < n0)%nat.
+  Proof.
+    inv MTCHST. inv STACK. ss. inv FINAL. inv AFTER. set WF as WF2. inv WF2. ss.
+    rewrite PCSAME in *. des. ss. clarify. esplits.
+    econs; simpl in *.
+    - eapply callee_save_agree; eauto.
+    - set unfree_free_inj.
+      specialize (i j m_src m1 m2 m_tgt blk blk0 0 (Ptrofs.unsigned ofs)).
+      eapply i; eauto. clear i.
+      rewrite INITRSP in RSPSAME. rewrite RSRSP0 in RSPSAME.
+      rewrite Ptrofs.repr_unsigned. auto.
+    - ss.
+    - ss. 
+    - ss.
+    - ss.
+    - des_ifs. omega.
+  Qed.
+
+  Lemma asm_step_preserve_injection
+        rs_src0 rs_src1 m_src0 m_src1 tr j0
+        rs_tgt0 m_tgt0
+        ge_src ge_tgt
+        (GENVLE: genv_le j0 ge_src ge_tgt)
+        (GE: genv_le j0 ge_src ge_tgt)
+        (AGREE: agree j0 rs_src0 rs_tgt0)
+        (INJ: Mem.inject j0 m_src0 m_tgt0)
+        (STEP: Asm.step ge_src (Asm.State rs_src0 m_src0) tr (Asm.State rs_src1 m_src1))
+    :
+      exists rs_tgt1 m_tgt1 j1,
+        (Asm.step ge_tgt (Asm.State rs_tgt0 m_tgt0) tr (Asm.State rs_tgt1 m_tgt1)) /\
+        (agree j1 rs_src1 rs_tgt1) /\
+        (Mem.inject j1 m_src1 m_tgt1) /\
+        (inject_incr j0 j1).
+  Admitted.
+
+  Lemma asm_step_internal_simulation
+        st_src0 st_src1 st_tgt0 tr frs p b0 b1 init_rs n0
+        (STEP: Asm.step (local_genv p) st_src0 tr st_src1)
+        (STEPRET: AsmC.step_ret skenv_link p st_src0 b1)
+        (MTCHST: match_states (State ((Frame.mk (AsmC.modsem skenv_link p)
+                                                (AsmC.mkstate init_rs st_src0 b0))::frs))
+                              st_tgt0 n0)
+    :
+      exists st_tgt1 n1,
+        Asm.step tge st_tgt0 tr st_tgt1 /\
+        match_states (State ((Frame.mk (AsmC.modsem skenv_link p)
+                                       (AsmC.mkstate init_rs st_src1 b1))::frs))
+                     st_tgt1 n1.
+  Proof.
+    inv MTCHST. apply asm_frame_inj in FRAME. inv FRAME. destruct st_src1.
+    exploit asm_step_preserve_injection; ss; eauto.
+    - apply local_genv_le. ss.
+    - apply local_genv_le; auto.
+    - ii. des. esplits; eauto; econs; eauto.
+      + etrans. apply INITINCR. auto.
+      + eapply match_stack_incr; eauto.
+  Qed.
+
+  Lemma step_internal_simulation
+        fr0 frs tr st0 st_tgt0 n0
+        (STEP: fr0.(Frame.ms).(ModSem.step) fr0.(Frame.ms).(ModSem.globalenv) fr0.(Frame.st) tr st0)
+        (MTCHST: match_states (State (fr0 :: frs)) st_tgt0 n0) 
+    :
+      exists st_tgt1 n1,
+        Asm.step tge st_tgt0 tr st_tgt1 /\
+        match_states (State ((fr0.(Frame.update_st) st0) :: frs)) st_tgt1 n1.
+  Proof.
+    inv MTCHST. inv STEP.
+    exploit asm_step_internal_simulation; ss; eauto.
+    - econs; eauto.
+    - ii. des. esplits; ss; eauto.
+      destruct st0; ss; clarify. eassumption.
+    Unshelve. auto.
+  Qed.
+
+  Lemma step_call_simulation
+        fr0 frs args st_tgt n
+        (AT: fr0.(Frame.ms).(ModSem.at_external) fr0.(Frame.st) args)
+        (MTCHST: match_states (State (fr0 :: frs)) st_tgt n)
+    :
+        match_states (Callstate args (fr0 :: frs)) st_tgt 1%nat.
+  Proof.
+    inv MTCHST. ss. inv AT.
+    econs; ss; eauto.
+    econs; eauto.
+  Qed.
+
+  Lemma to_fake_fake_ptr v : ~ is_real_ptr (to_fake v).
+  Proof.
+    intros i. inv i. destruct v; ss. destruct b0; ss.
+  Qed.
+
+  Lemma nextblock_unvalid j m1 m2
+        (INJ: Mem.inject j m1 m2)
+    :
+      j (Mem.nextblock m1) = None.
+  Proof.
+    inv INJ. eapply mi_freeblocks.
+    unfold Mem.valid_block. apply Plt_strict.
+  Qed.
+
+  Lemma callee_injection_incr j old_blk new_blk delta
+        (INJ_NONE: j new_blk = None)
+    :
+      inject_incr j (callee_injection j old_blk new_blk delta).
+  Proof.
+    unfold callee_injection. ii. des_ifs.
+  Qed.
+
+  Lemma memcpy_inject j m_src m_tgt blk ofs size 
+        (INJ: Mem.inject j m_src m_tgt)
+    :
+      Mem.inject (callee_injection j blk (Mem.nextblock m_src) ofs)
+                 (memcpy m_src blk ofs size) m_tgt.
+  Admitted.
+
+  Lemma local_genv_skenv_signature p fptr fd
+        (FIND: Genv.find_funct (local_genv p) fptr = Some (Internal fd))
+    :
+      Genv.find_funct skenv_link fptr = Some (Internal (fn_sig fd)).
+  Admitted.
+
+  Lemma src_init_rs_PTRFREE sg rs v
+    :
+      forall
+          pr mr
+          (MR: to_mreg pr = Some mr)
+          (NOTIN: ~In (R mr) (regs_of_rpairs (loc_arguments sg)))
+        ,
+          <<PTRFREE: ~ is_real_ptr ((src_init_rs sg rs v) pr)>>.
+  Proof.
+    i. intros PTR. unfold src_init_rs in PTR.
+    des_ifs; eapply to_fake_fake_ptr; eauto.
+  Qed.
+
+  Lemma skenv_link_main
+    :
+      Genv.find_funct
+        skenv_link (Genv.symbol_address tge (prog_main tprog) Ptrofs.zero)
+      = Some (Internal signature_main).
+  Admitted.
+
+  Lemma src_init_rs_arguments (rs: regset) m0 m1 sg rsp mr v
+        (ARG: extcall_arg rs m0 (R mr) v)
+        (IN: In (R mr) (regs_of_rpairs (loc_arguments sg)))
+    :
+      extcall_arg (src_init_rs sg rs rsp) m1 (R mr) v.
+  Proof.
+    inv ARG.
+    replace (rs (preg_of mr)) with (src_init_rs sg rs rsp (preg_of mr)); [econs|].
+    unfold src_init_rs.
+    destruct mr; ss; des_ifs.
+  Qed.
+
+  Lemma memcpy_property m0 m1 m2 blk lo size
+        (FREE: m0.(Mem.free) blk lo (lo + size) =
+               Some m1)
+        (ALLOC: Mem.alloc m1 0 size = (m2, m0.(Mem.nextblock)))
+    :
+      Mem.unchanged_on
+        (fun blk0 ofs0 => if eq_block blk0 (m0.(Mem.nextblock)) then ~ (0 <= ofs0 < size) else True)
+        m2 (memcpy m0 blk lo size).
+  Proof.
+    econs.
+    - rewrite memcpy_spec1.
+      erewrite Mem.nextblock_alloc; eauto.
+      erewrite Mem.nextblock_free; eauto.
+      reflexivity.
+    - intros blk0 ofs0 k p EQ VALID.
+      des_ifs.
+      + split; intro PERM.
+        * eapply Mem.perm_alloc_3 in PERM; eauto. clarify.
+        * eapply memcpy_spec3_2 in PERM; clarify.
+      + split; intro PERM; destruct (eq_block blk0 blk); clarify.
+        * admit "".
+        * eapply memcpy_spec3_3; auto.
+          eapply Mem.perm_alloc_4 in PERM; [| apply ALLOC| eauto].
+          eapply Mem.perm_free_3; eauto.
+        * admit "".
+        * erewrite memcpy_spec3_3 in PERM; eauto.
+          eapply Mem.perm_alloc_1; eauto.
+          eapply Mem.perm_free_1; eauto.
+    - intros blk0 ofs0 EQ PERM. des_ifs.
+  Admitted.
+
+  Lemma memcpy_arguments (rs0 rs1: regset) m sg blk ofs delta ty v
+        (RSRSP0: rs0 # RSP = Vptr blk ofs true)
+        (REPRESENT:
+           Ptrofs.unsigned ofs + (4 * size_arguments sg) <= Ptrofs.modulus)
+        (RSRSP1: rs1 # RSP = Vptr (Mem.nextblock m) Ptrofs.zero true)
+        (ARG: extcall_arg rs0 m (S Outgoing delta ty) v)
+        (DELTA: 0 <= delta < size_arguments sg)
+    :
+      extcall_arg
+        rs1
+        (memcpy m blk (Ptrofs.unsigned ofs)
+                (4 * size_arguments sg)) (S Outgoing delta ty) v.
+  Proof.
+    econs. reflexivity. inv ARG. rewrite RSRSP0 in *. rewrite RSRSP1 in *. ss.
+    rewrite Ptrofs.add_zero_l. rewrite memcpy_load.
+    - replace (Ptrofs.unsigned ofs + Ptrofs.unsigned (Ptrofs.repr (4 * delta)))
+        with (Ptrofs.unsigned (Ptrofs.add ofs (Ptrofs.repr (4 * delta)))); auto.
+      admit "ez".
+    - rewrite Ptrofs.unsigned_repr; [omega|].
+      split; try omega.
+      admit "ez".
+  Qed.
+
+  Lemma free_success m0 blk lo hi m1
+        (FREE: Mem.free m0 blk lo hi = Some m1)
+    :
+      Mem.range_perm m0 blk lo hi Cur Freeable.
+  Proof.
+    Local Transparent Mem.free. unfold Mem.free in FREE. des_ifs; eauto.
+  Qed.
+
+  Lemma memcpy_store_arguments rs m0 m1 sg args blk ofs true
+        (ARGS: extcall_arguments rs m0 sg args)
+        (RSRSP: rs # RSP = Vptr blk ofs true)
+        (FREE: Mem.free m0 blk (Ptrofs.unsigned ofs) (Ptrofs.unsigned ofs + 4 * size_arguments sg) = Some m1)
+    :
+      store_arguments
+        m1
+        (src_init_rs sg rs (Vptr (Mem.nextblock m0) Ptrofs.zero true))
+        args sg (memcpy m0 blk (Ptrofs.unsigned ofs) (4 * size_arguments sg)).
+  Proof.
+    destruct (Mem.alloc m1 0 (4 * size_arguments sg)) eqn:MEQ.
+    destruct (eq_sym (Mem.alloc_result _ _ _ _ _ MEQ)).
+    erewrite Mem.nextblock_free in MEQ; eauto.
+    econs; eauto.
+    - admit "".
+    - eapply memcpy_property; eauto.
+    - rewrite memcpy_spec1.
+      erewrite Mem.nextblock_alloc; [|eauto].
+      erewrite Mem.nextblock_free; eauto.
+    - intros ofs0 BOUND.
+      apply memcpy_spec3_1; auto.
+      eapply free_success; eauto. omega.
+  Qed.    
+  
+  Lemma step_init_simulation
+        args frs st_tgt p fd n
+        (MTCHST: match_states (Callstate args frs) st_tgt n)
+        (MSFIND: ge.(Ge.find_fptr_owner) args.(Args.fptr) (AsmC.modsem skenv_link p))
+        (FINDF: Genv.find_funct (local_genv p) args.(Args.fptr) = Some (Internal fd))
+        (SIZEWF: 4 * size_arguments (fn_sig fd) <= Ptrofs.modulus)
+    :
+      exists rs m,
+        (AsmC.initial_frame skenv_link p args (AsmC.mkstate rs (Asm.State rs m) false)) /\
+        (match_states (State ((Frame.mk (AsmC.modsem skenv_link p) (AsmC.mkstate rs (Asm.State rs m) false)) :: frs)) st_tgt 0).
+  Proof.
+    inv MTCHST. des. ss. set (nextblock_unvalid := nextblock_unvalid INJECT).
+    set (SKDSG:= local_genv_skenv_signature _ _ FINDF). clarify.
+    exists (src_init_rs (fn_sig fd) init_rs (Vptr m_src.(Mem.nextblock) Ptrofs.zero true)).
+    exists (memcpy m_src blk (Ptrofs.unsigned ofs) (4 * size_arguments (fn_sig fd))).
+    esplits; eauto.
+    - econs.
+      + apply (eq_refl (fn_sig fd)).
+      + apply FINDF.
+      + ss.
+      + unfold src_init_rs. ss. f_equal.
+        symmetry. eapply Mem.nextblock_free. eauto.
+      + ss.
+      + eapply memcpy_store_arguments; eauto.
+      + apply src_init_rs_PTRFREE.
+    - econs.
+      + instantiate (2 := callee_injection j blk (Mem.nextblock m_src) (Ptrofs.unsigned ofs)).
+        eapply src_init_rs_agree; eauto.
+        apply Ptrofs.repr_unsigned.
+      + instantiate (1 := memcpy m_src blk (Ptrofs.unsigned ofs)
+                                 (4 * size_arguments (fn_sig fd))).
+        eapply memcpy_inject; auto.
+      + eapply inject_incr_trans with (f2 := j); auto.
+        apply callee_injection_incr; auto.
+      + reflexivity.
+      + inv STACK; econs; ss; [apply skenv_link_main| |].
+        * eapply match_stack_incr; [|eauto].
+          apply callee_injection_incr; auto.
+        * set (AGREERSP := AGREE RSP).
+          rewrite RSPPTR in AGREERSP. inv AGREERSP.
+          eapply src_init_rs_wf; eauto.
+      + unfold external_state.
+        des_ifs. exfalso. unfold src_init_rs, local_genv in *. ss.
+        rewrite <- FPTR in *. rewrite Heq0 in *. ss. des_ifs.
+        clear - FINDF Heq1. remember (SkEnv.revive (SkEnv.project skenv_link (defs p)) p).
+        unfold fundef in *. clarify.
+  Qed.
+
+  Definition index := nat.
+
+  Definition order := le.
+
+  Lemma symb_preserved id
+    :
+      Senv.public_symbol (symbolenv (semantics tprog)) id =
+      Senv.public_symbol (symbolenv (sem prog)) id.
+  Admitted.
+
+  Lemma at_external_external p st frs st_tgt n args
+        (MTCHST: match_states
+                   (State
+                      ((Frame.mk (AsmC.modsem skenv_link p) st)::frs))
+                   st_tgt n)
+        (ATEXTERNAL: at_external skenv_link p st args)
+    :
+      (1 < n)%nat.
+  Proof.
+    inv MTCHST.
+    replace (at_external skenv_link p) with (at_external skenv_link p0) in *.
+    - inv ATEXTERNAL. apply asm_frame_inj in FRAME. clarify.
+      unfold external_state. des_ifs. omega.
+    - apply f_equal with (f := Frame.ms) in FRAME. ss.
+      inv FRAME. apply Eqdep.EqdepTheory.inj_pair2 in H1. auto.
+  Qed.  
+
+  Lemma normal_state_fsim_step frs st_src1 st_tgt0 t n0
+        (MTCHST: match_states (State frs) st_tgt0 n0)
+        (STEP: step ge (State frs) t st_src1)
+    :
+      (exists st_tgt1 n1,
+          Asm.step tge st_tgt0 t st_tgt1 /\ match_states st_src1 st_tgt1 n1) \/
+      (exists n1,
+          match_states st_src1 st_tgt0 n1 /\ n1 < n0)%nat /\ (t = E0).
+  Proof.
+    inv STEP.
+    - right. exploit step_call_simulation; eauto.
+      i. esplits; eauto.
+      inv MTCHST; ss.
+      exploit at_external_external; eauto.
+      econs; try eassumption; ss.
+    - left. exploit step_internal_simulation; eauto.
+    - right. exploit step_return_simulation; eauto.
+  Qed.
+
+  Lemma match_state_xsim
+    :
+      forall st_src st_tgt n (MTCHST: match_states st_src st_tgt n),
+        xsim (sem prog) (semantics tprog) lt n st_src st_tgt.
+  Proof.
+    pcofix CIH. i. pfold. destruct st_src.
+    - admit "init".
+    - left. econs.
+      + i. econs.
+        * exploit transf_final_states; eauto.
+        * { (** D return **)
+            i. inv FINAL0. inv FINAL1. eq_closure_tac.
+          }
+        * ii. inv FINAL. inv H; eq_closure_tac.
+      + econs.
+        * i. ss. rewrite LINK_SK in *.
+          exploit normal_state_fsim_step; eauto.
+          i. des; esplits; eauto.
+          -- left. econs; ss.
+             ++ econs; eauto. admit "determinate at".
+             ++ econs 1.
+             ++ rewrite E0_right. auto.
+          -- right. econs; ss. clarify. econs.
+        * admit "receptive at".
+  Qed.
+  
+  Lemma transf_xsim_properties
+    :
+        xsim_properties (sem prog) (semantics tprog) nat lt.
+  Proof.
+    econs; [apply lt_wf| |apply symb_preserved].
+    econs. i.
+    exploit (transf_initial_states); eauto.
+    i. des. esplits. econs; eauto.
+    - { (** D init **)
+        i. inv INIT0. inv INIT1. clarify.
+      }
+    - apply match_state_xsim; eauto.
+  Qed.
+
+  Lemma transf_program_correct:
+    mixed_simulation (Sem.sem prog) (Asm.semantics tprog).
+  Proof.
+    eapply Mixed_simulation. eapply transf_xsim_properties.
+  Qed.    
+
+End PRESERVATION.
