cfrontend/UpperBound_B1.v
@@ -1,0 +1,72 @@
+Require Import CoqlibC Maps.
+Require Import ASTC Integers Floats Values MemoryC Events Globalenvs Smallstep.
+Require Import Locations Stacklayout Conventions Linking.
+(** newly added **)
+Require Export Csem Cop Ctypes Ctyping Csyntax Cexec.
+Require Import Simulation Memory ValuesC.
+Require Import Skeleton ModSem Mod sflib.
+Require Import CtypesC CsemC Sem Syntax LinkingC Program.
+
+Set Implicit Arguments.
+
+Local Opaque Z.mul.
+
+Section PRESERVATION.
+
+  Existing Instance Val.mi_final.
+
+(** PLAN B-0*)
+
+(*
+B-0
+* : Physical
++ : Logical 
+c0 * empty
+>=
+c0 + empty
+*)
+  
+(*
+B-1
+* : Physical
++ : Logical 
+(c0 * c1) * ctx
+>=
+(c0 + c1) * ctx
+*)
+
+  Section PLANB1.
+
+(** ********************* linking *********************************)    
+  Variable prog1 : Csyntax.program.
+  Variable prog2 : Csyntax.program.
+  Variable prog' : Csyntax.program.
+  Hypothesis LINK : link prog1 prog2 = Some prog'.
+  Let tprog' : Syntax.program := List.map CsemC.module [prog2; prog1].
+  Variable ctx : Syntax.program.
+
+  Let prog : Syntax.program := CsemC.module prog' :: ctx.
+  Let tprog : Syntax.program := tprog' ++ ctx.
+
+(** ********************* linking *********************************)
+
+  Variable sk_src: Sk.t.
+  Hypothesis LINK_SK_SRC: link_sk prog = Some sk_src.
+  (* TODO: consider linking fail case *)
+  Let skenv_link_src := Sk.load_skenv sk_src.
+
+  Variable sk_tgt: Sk.t.
+  Hypothesis LINK_SK_TGT: link_sk tprog = Some sk_tgt.
+  (* TODO: consider linking fail case *)
+  Let skenv_link_tgt := Sk.load_skenv sk_tgt.
+  
+  Let ge := load_genv prog skenv_link_src.
+  (* Let ge_ce : composite_env := prog_comp_env prog. *)
+  (* Let tge_ce : composite_env := prog_comp_env prog. *)
+  Let tge := load_genv tprog skenv_link_tgt.
+
+  Inductive match_states_aux : Csem.State -> Sem.state -> nat -> Prop :=
+  
+  Inductive match_states : Sem.state -> Sem.state -> nat -> Prop :=
+  | match_states_intro
+      
